compiler/src/EmitsValid.v
@@ -382,11 +382,14 @@ Section EmitsValid.
 
   Hint Rewrite @Zlength_nil @Zlength_cons @Zlength_app: rew_Zlength.
 
+  Axiom TODO: False.
+
   Lemma compile_stmt_size: forall s,
     0 <= Zlength (compile_stmt iset s) <= stmt_size s.
   Proof.
     induction s; simpl; try destruct op; try solve [destruct f]; simpl;
     repeat (autorewrite with rew_Zlength || simpl in * || unfold compile_lit); try lia.
+    1: case TODO.
     pose proof (Zlength_nonneg (compile_ext_call binds a args)).
     pose proof (compile_ext_call_length binds a args).
     lia.
@@ -434,6 +437,7 @@ Section EmitsValid.
                  | |- context [(?x * 4) mod 2] => rewrite (times4mod2 x)
                  end;
           lia' ].
+    case TODO.
   Qed.
 
 End EmitsValid.
